hashNodes implementation using abstracted update b nodes

src/IsoCan.v
@@ -16,9 +16,9 @@ Section IsoCan.
   Let term_countType_ := (term_countType I B L).
   Let is_bnode := (@is_bnode I B L).
 
-  Definition isocanonical_function (M : B -> B) (g : rdf_graph_) :=
+(*   Definition isocanonical_function (M : B -> B) (g : rdf_graph_) :=
     iso g (Rdf.relabeling M g) /\
-      forall (h : rdf_graph_), iso g h <-> (relabeling M g) = (relabeling M h).
+      forall (h : rdf_graph_), iso g h <-> (relabeling M g) = (relabeling M h). *)
 
   Section IsoCanAlgorithm.
     Variable h : countType.
@@ -34,49 +34,28 @@ Section IsoCan.
     Definition hash_canPOrderMixin := PcanPOrderMixin (@pickleK hash_countType).
     Canonical hash_POrderType := Eval hnf in POrderType tt h hash_canPOrderMixin.
     Variable hashTerm : term_ -> h.
+    Section Hash.
+    Variable T : countType.
 
     Record hi_term := mkHinput {
-                         input : term_ ;
+                         input : T ;
                          current_hash : h
                        }.
+
 
 
     Hypothesis perfectHashingSchemeTerm : injective hashTerm.
 
     Lemma by_perf_hash (i : term_) (o : h) (eqb : hashTerm i == o) : hashTerm i = o. apply /eqP. apply eqb. Qed.
 
-    (* Definition hi_term_inj_o (hin1 hin2: hi_term): *)
-    (*   output hin1 = output hin2 -> *)
-    (*   hin1 = hin2. *)
-    (* Proof. case: hin1; case: hin2 => [i1 o1 io1] i2 o2 io2 /= oeq.  *)
-    (*        have ieq : i1 = i2. *)
-    (*        apply perfectHashingSchemeTerm; apply /eqP; by rewrite (by_perf_hash io1) (by_perf_hash io2) oeq. *)
-    (*        subst. by f_equal; apply eq_irrelevance. *)
-    (* Qed. *)
-
-    (* Definition hi_term_inj_i (hin1 hin2: hi_term): *)
-    (*   input hin1 = input hin2 -> *)
-    (*   hin1 = hin2. *)
-    (* Proof. case: hin1; case: hin2 => [i1 o1 io1] i2 o2 io2 /= ieq. subst. *)
-    (*        have io1P: hashTerm i1 = o1. apply /eqP. apply io1. *)
-    (*        have io2P: hashTerm i1 = o2. apply /eqP. apply io2. subst. f_equal. apply eq_irrelevance. *)
-    (* Qed. *)
-
-    Definition code_hash (x : hi_term) :=
+    Definition code_hash (x : hi_term) : GenTree.tree nat :=
       let (i,o) := x in
       GenTree.Node 0 [:: GenTree.Leaf (pickle i); GenTree.Leaf (pickle o)].
 
-    (* Definition build_hash (i : term) : option hi_term. *)
-    (* Proof. *)
-    (*   (* have o: h. exact (hashTerm i). *) *)
-    (*   have E : hashTerm i == hashTerm i. by []. *)
-    (*   - exact (Some (mkHinput E)). *)
-    (* Defined. *)
-
-    Definition decode_hash (x : GenTree.tree nat) : option hi_term:=
+    Definition decode_hash (x : GenTree.tree nat) : option hi_term :=
       match x with
       | GenTree.Node 0 [:: GenTree.Leaf n; GenTree.Leaf m] =>
-          match (@unpickle term_countType_ n, @unpickle hash_countType m) with
+          match (@unpickle T n, @unpickle hash_countType m) with
           | (Some i, Some o) => Some (mkHinput i o)
           | (_, _) => None
           end
@@ -84,7 +63,7 @@ Section IsoCan.
       end.
 
     Definition cancel_hin_encode : pcancel code_hash decode_hash.
-    Proof. case => i o. rewrite /code_hash /decode_hash. by rewrite !pickleK. Qed.
+    Proof. case => i o; by rewrite /code_hash /decode_hash !pickleK. Qed.
 
     Definition hin_eqMixin := PcanEqMixin cancel_hin_encode.
     Definition hin_canChoiceMixin := PcanChoiceMixin cancel_hin_encode.
@@ -92,21 +71,23 @@ Section IsoCan.
 
     Canonical hin_eqType := Eval hnf in EqType hi_term hin_eqMixin.
     Canonical hin_choiceType := Eval hnf in ChoiceType hi_term hin_canChoiceMixin.
-    Canonical hin_countType := Eval hnf in CountType hi_term hin_canCountMixin.
-    Definition hin_canPOrderMixin := PcanPOrderMixin (@pickleK hin_countType).
+    Canonical hin_ct := Eval hnf in CountType hi_term hin_canCountMixin.
+    Definition hin_canPOrderMixin := PcanPOrderMixin (@pickleK hin_ct).
     Canonical hin_POrderType := Eval hnf in POrderType tt hi_term hin_canPOrderMixin.
 
     Definition hash := hi_term.
+    End Hash.
+    
+    Definition eqb_t_hi (t : term_) (ht : term I (hin_ct B) L) : bool :=
+      match t, ht with
+      | Iri i, Iri i' => i == i'
+      | Bnode b,Bnode hin => b == (input hin)
+      | Lit l, Lit l' => l == l'
+      | _,_ => false
+      end.
 
-    (* Definition initTerm (t : term) : hash := *)
-    (*   match t with *)
-    (*   | Bnode name => None *)
-    (*   | otherwise => Some (hi_term t) end. *)
+(*     Definition hashmap := seq hash. *)
 
-    Definition hashmap := seq hash.
-
-    (* Definition initHashMap (g : rdf_graph) : hashmap := map initTerm (terms g). *)
-    (* Variable doHash (g : rdf_graph) (hm : hashmap) (hm : seq hashmap) (n : nat) -> seq hashmap. *)
     Section typeRelabel.
       Variable T : countType.
 
@@ -118,11 +99,11 @@ Section IsoCan.
         end.
 
       Definition app_p_sib (s : term I B L) (f : B -> T) : (is_in_ib s) -> (is_in_ib (app_term s f)).
-      Proof. rewrite /app_term. case s; by []. Qed.
+      Proof. rewrite /app_term; by case s. Qed.
       Definition app_p_pii (p : term I B L) (f : B -> T) : (is_in_i p) -> (is_in_i (app_term p f)).
-      Proof. rewrite /app_term. case p; by []. Qed.
+      Proof. rewrite /app_term; by case p. Qed.
       Definition app_p_ibl (o : term I B L) (f : B -> T) : (is_in_ibl o) -> (is_in_ibl (app_term o f)).
-      Proof. rewrite /app_term. case o; by []. Qed.
+      Proof. rewrite /app_term; by case o. Qed.
 
       Definition MoveTriple (f : B -> T) (t : triple I B L) : triple I T L :=
         let (s,p,o,sin,pin,oin) := t in
@@ -138,38 +119,206 @@ Section IsoCan.
       Definition hash_graph (g : seq (triple I B L)) (f : B -> T): seq (triple I T L) :=
         map (MoveTriple f) g.
 
-  Lemma app_st_p_sin (g : seq (triple I B L) ) (f : B -> T) :
-    all (fun t => is_in_ib (subject t)) g ->
-    all (fun t => is_in_ib (subject t)) (hash_graph g f).
-  Proof. move=> /allP sin. apply /allP => [[s p o /= sint pint oint]] => tg. by apply sint. 
-  Qed.
+      Lemma app_st_p_sin (g : seq (triple I B L) ) (f : B -> T) :
+        all (fun t => is_in_ib (subject t)) g ->
+        all (fun t => is_in_ib (subject t)) (hash_graph g f).
+      Proof. move=> /allP sin; apply /allP => [[s p o /= sint pint oint]] => tg; by apply sint. 
+      Qed.
 
-  Lemma app_st_p_pin (g : seq (triple I B L)) (μ : B -> T) :
-    all (fun t => is_in_i (predicate t)) g ->
-    all (fun t => is_in_i (predicate t)) (hash_graph g μ).
-  Proof. move=> /allP pin. apply /allP => [[s p o /= sint pint oint]] => tg. by apply pint.
-  Qed.
+      Lemma app_st_p_pin (g : seq (triple I B L)) (μ : B -> T) :
+        all (fun t => is_in_i (predicate t)) g ->
+        all (fun t => is_in_i (predicate t)) (hash_graph g μ).
+      Proof. move=> /allP pin; apply /allP => [[s p o /= sint pint oint]] => tg; by apply pint.
+      Qed.
 
-  Lemma app_st_p_oin (g : seq (triple I B L)) (μ : B -> T) :
-    all (fun t => is_in_ibl (object t)) g ->
-    all (fun t => is_in_ibl (object t)) (hash_graph g μ).
-  Proof. move=> /allP oin. apply /allP => [[s p o /= sibt pibt oint]] => tg. by apply oint.
-  Qed.
+      Lemma app_st_p_oin (g : seq (triple I B L)) (μ : B -> T) :
+        all (fun t => is_in_ibl (object t)) g ->
+        all (fun t => is_in_ibl (object t)) (hash_graph g μ).
+      Proof. move=> /allP oin; apply /allP => [[s p o /= sibt pibt oint]] => tg; by apply oint.
+      Qed.
 
-    Definition graph_map (f : B -> T) (g : rdf_graph_): rdf_graph I T L:=
-      let (g',sin,pin,oin) := g in
-      mkRdfGraph (app_st_p_sin f sin)(app_st_p_pin f pin) (app_st_p_oin f oin).
+      Definition graph_map (f : B -> T) (g : rdf_graph_): rdf_graph I T L:=
+        let (g',sin,pin,oin) := g in
+        mkRdfGraph (app_st_p_sin f sin)(app_st_p_pin f pin) (app_st_p_oin f oin).
 
     End typeRelabel.
+    
+    Definition get_triple (t : term I B L) (trpl : triple I (hin_ct B) L) : option (term I (hin_ct B) L) :=
+      let (s,p,o,_,_,_) := trpl in
+      if eqb_t_hi t s then Some s
+      else if eqb_t_hi t p then Some p
+      else if eqb_t_hi t o then Some o
+      else None.
+      
+    Definition is_some {T : Type} (ot : option T) : bool := 
+      match ot with Some _ => true | None => false end.
+
+    Definition get (t : term_) (g : rdf_graph I (hin_ct B) L) : option (term I (hin_ct B) L) :=
+      let otrs := (map (get_triple t) (graph g)) in
+      head None (filter is_some otrs).
+
+(*     Definition lookup_hash (g : rdf_graph I (hin_ct B) L) (b : term I B L): option (hash B) :=
+      let ot := get b g in
+      match ot with 
+      | Some (Bnode hin) => Some hin
+      | _ => None
+      end. *)
+
+    Definition lookup_hash (b : term I (hin_ct B) L): option (hash B) :=
+      match b with 
+      | Bnode hin => Some hin
+      | _ => None
+      end.
 
 
-    Definition init_bnode (b : B) : hi_term :=
-      mkHinput (Bnode I L b) h0.
+      Section Partition.
 
-    Definition init_hash (g : rdf_graph_) : rdf_graph I hin_countType L :=
-      graph_map init_bnode g.
+(*     Definition eq_rel (g : rdf_graph I (hin_ct B) L) (b1 b2 : term I B L ) : bool :=
+      match (lookup_hash b1), (lookup_hash b2) with
+      | Some hin1, Some hin2 => current_hash hin1 == current_hash hin2
+      | _,_ => false
+      end. *)
 
-(*     Variable hashNodes : (rdf_graph -> seq hashmap).
+    Definition eq_rel (b1 b2 : term I (hin_ct B) L ) : bool :=
+      match (lookup_hash b1), (lookup_hash b2) with
+      | Some hin1, Some hin2 => current_hash hin1 == current_hash hin2
+      | _,_ => false
+      end.
+
+    Fixpoint partitionate (f : (term I (hin_ct B) L) -> bool) (s:seq (term I (hin_ct B) L)) : list (term I (hin_ct B) L) * list (term I (hin_ct B) L) :=
+      match s with
+      | nil => (nil, nil)
+      | x :: tl => let (g,d) := partitionate f tl in
+                 if f x then (x::g,d) else (g,x::d)
+      end.
+
+    Definition part := seq (hash B).
+    Definition partition := seq part.
+
+    Fixpoint unwrap {T : Type} (os : seq (option T)) : seq T :=
+      match os with
+      | nil => nil
+      | Some t :: oss => t :: unwrap oss
+      | None :: oss => unwrap oss
+      end.
+
+    Definition mkPartition (g : rdf_graph I (hin_ct B) L) : partition :=
+      let bns := (bnodes g) in
+      let equiv := (fun b => (fun t=> eq_rel b t)) in
+      let P := undup (map (fun b=> (partitionate (equiv b) bns).1 ) bns) in
+      let ohs := map (fun bs => map lookup_hash bs) P in
+      map unwrap ohs.
+
+    Record Partition := mkPartition_ {
+                           P : partition ;
+                           g : rdf_graph I (hin_ct B) L ;
+                           p_wf : P == mkPartition g  ;
+                           has_b : all (fun p=> ~~ (nilp p)) P ;
+                           diff_hashes : uniq P 
+
+                         }.
+
+    (* Error: Cannot guess decreasing argument of fix. *)
+    (* Definition mkPartition (g : rdf_graph) (hm : hashmap) := *)
+    (*   let fix part (bnodes : seq term) (acc : seq (seq term)) := *)
+    (*                match bnodes with *)
+    (*                | nil => acc *)
+    (*                | b :: bs => *)
+    (*                    let equiv := (fun t=> eq_rel g hm b t) in *)
+    (*                    let (a_part,rest) := partition equiv bs in *)
+    (*                    part rest (a_part::acc) *)
+    (*                end in *)
+    (*   part (bnodes g) hm [::]. *)
+
+    (* Definition mkPartition (g : rdf_graph) (hm : hashmap) := *)
+    (*   let fix aux (bnodes : seq term) (acc : seq (seq term)) := *)
+    (*                match bnodes with *)
+    (*                | nil => acc *)
+    (*                | b :: bs => *)
+    (*                    let equiv := (fun t=> eq_rel g hm b t) in *)
+    (*                    let part := filter equiv bs in *)
+    (*                    let rest := foldr (@rem (term_eqType I B L)) bs part in *)
+    (*                    aux rest (part::acc) *)
+    (*                    (* aux (filter (fun t=>(~~ (equiv t))) bs) (part::acc) *) *)
+    (*                end in *)
+    (*   aux (bnodes g) hm [::]. *)
+
+    (* Record partition := mkPartition { *)
+    (*                        bnodes : seq term ; *)
+    (*                        bnodes_r_bnodes : all is_bnode bnodes ; *)
+    (*                        hm : hashmap ; *)
+
+
+    (*                      }. *)
+
+    Definition is_trivial (part : part) : bool :=
+      size part == 1.
+
+    Definition is_non_trivial (part : part) : bool :=
+      ~~ is_trivial part.
+
+    Definition is_fine (p : partition) : bool :=
+      all is_trivial p.
+
+    Definition is_coarse (p : partition) : bool :=
+      size p == 1.
+
+    Definition is_intermediate (p : partition) :=
+      ~~ is_fine p && ~~ is_coarse p.
+
+
+
+    (* Definition lt_part (part1 part2 : part) : bool := *)
+    (*   if size part1 < size part2 then *)
+    (*     true *)
+    (*   else if size part1 == size part2 then *)
+
+
+    (*          Definition le_partition (p1 p2 : partition) : bool :=  *)
+    (*          fun T : Type => T -> pred T *)
+    (*                                eq_refl. *)
+    (*          . *)
+    (*          Definition partition_LePOrderMixin := LePOrderMixin partition. *)
+    (*          forall (T : eqType) (le lt : rel T), *)
+    (*   (forall x y : T, lt x y = (y != x) && le x y) -> *)
+    (*   reflexive le -> antisymmetric le -> transitive le -> lePOrderMixin T *)
+
+    
+  End Partition. 
+
+
+
+  Definition init_bnode (b : B) : (hi_term B) :=
+    mkHinput b h0.
+
+  Definition init_hash (g : rdf_graph_) : rdf_graph I (hin_ct B) L :=
+    graph_map init_bnode g.
+
+  Definition cmp_part (p1 p2 : part) : bool :=
+    all2 (fun b1 b2 => input b1 == input b2) p1 p2.
+
+  Definition partition_didnt_change (g h: rdf_graph I (hin_ct B) L) : bool :=
+    let pg := mkPartition g in 
+    let ph := mkPartition h in
+    all2 (fun p1 p2 => cmp_part p1 p2) pg ph.
+
+  Variable update_bnodes : rdf_graph I (hin_ct B) L -> rdf_graph I (hin_ct B) L.
+
+  Fixpoint iterate (g h: rdf_graph I (hin_ct B) L) (fuel : nat) : rdf_graph I (hin_ct B) L :=
+    match fuel with
+    | O => h 
+    | S n' =>
+      if partition_didnt_change g h then h else
+      let g' := update_bnodes h in
+      iterate h g' n'
+      end.
+
+  Definition hashNodes (g : rdf_graph_ ) : (rdf_graph I (hin_ct B) L) :=
+    let ini := init_hash g in
+    let iter := update_bnodes ini in
+    iterate ini iter (size (graph g)).
+
+      (*     Variable hashNodes : (rdf_graph -> seq hashmap).
     Variable lookup_hashmap : (hashmap -> term -> hash).
 
     Hypothesis hash_dont_get_equal :
@@ -190,117 +339,16 @@ Section IsoCan.
              (c : term) (cinh : c \in (bnodes (h))),
       exists μ, (relabeling_term μ b) = c -> lookup_hashmap hash_g b = lookup_hashmap hash_h c. *)
 
-    (* Hypothesis perfectHashingSchemeTriple : injective hashTriple. *)
+      (* Hypothesis perfectHashingSchemeTriple : injective hashTriple. *)
 
-    Variable hashBag : (seq hash -> hash).
-    Hypothesis hashBag_assoc : forall (l l1 l2 l3: seq hash) (perm : l = l1 ++ l2 ++ l3),
-        hashBag ([:: hashBag (l1 ++ l2)] ++ l3) = hashBag (l1 ++ [:: hashBag (l2 ++ l3)]).
-    Hypothesis hashBag_comm : forall (l l1 l2: seq hash) (perm : l = l1 ++ l2),
-        hashBag l = hashBag (l2 ++ l1).
+      Variable hashBag : (seq hash -> hash).
+  Hypothesis hashBag_assoc : forall (l l1 l2 l3: seq hash) (perm : l = l1 ++ l2 ++ l3),
+      hashBag ([:: hashBag (l1 ++ l2)] ++ l3) = hashBag (l1 ++ [:: hashBag (l2 ++ l3)]).
+  Hypothesis hashBag_comm : forall (l l1 l2: seq hash) (perm : l = l1 ++ l2),
+      hashBag l = hashBag (l2 ++ l1).
 
-(*     Section Partition.
-
-      Definition eq_rel (g : rdf_graph) (hm : hashmap) (b1 b2 : term) : bool :=
-        (b1 \in (bnodes g)) && (b2 \in (bnodes g)) && (lookup_hashmap hm b1 == lookup_hashmap hm b2).
-
-      Check partition.
-
-      Fixpoint partitionate {A : Type} (f : A -> bool) (s:seq A) : list A * list A :=
-        match s with
-        | nil => (nil, nil)
-        | x :: tl => let (g,d) := partitionate f tl in
-                     if f x then (x::g,d) else (g,x::d)
-        end.
-
-      Definition part := seq hash.
-      Definition partition := seq part.
-
-      Definition mkPartition (g : rdf_graph) (hm : hashmap) : partition :=
-        let bns := (bnodes g) in
-        let equiv := (fun b => (fun t=> eq_rel g hm b t)) in
-        let P := undup (map (fun b=> (partitionate (equiv b) bns).1 ) bns) in
-        map (fun bs => map (lookup_hashmap hm) bs) P.
-
-      Record Partition := mkPartition_ {
-                             P : partition ;
-                             g : rdf_graph ;
-                             hm : hashmap ;
-                             p_wf : P == mkPartition g hm ;
-                             has_b : all (fun p=> ~~ (nilp p)) P ;
-                             diff_hashes : uniq P 
-
-                           }.
-
-      (* Error: Cannot guess decreasing argument of fix. *)
-      (* Definition mkPartition (g : rdf_graph) (hm : hashmap) := *)
-      (*   let fix part (bnodes : seq term) (acc : seq (seq term)) := *)
-      (*                match bnodes with *)
-      (*                | nil => acc *)
-      (*                | b :: bs => *)
-      (*                    let equiv := (fun t=> eq_rel g hm b t) in *)
-      (*                    let (a_part,rest) := partition equiv bs in *)
-      (*                    part rest (a_part::acc) *)
-      (*                end in *)
-      (*   part (bnodes g) hm [::]. *)
-
-      (* Definition mkPartition (g : rdf_graph) (hm : hashmap) := *)
-      (*   let fix aux (bnodes : seq term) (acc : seq (seq term)) := *)
-      (*                match bnodes with *)
-      (*                | nil => acc *)
-      (*                | b :: bs => *)
-      (*                    let equiv := (fun t=> eq_rel g hm b t) in *)
-      (*                    let part := filter equiv bs in *)
-      (*                    let rest := foldr (@rem (term_eqType I B L)) bs part in *)
-      (*                    aux rest (part::acc) *)
-      (*                    (* aux (filter (fun t=>(~~ (equiv t))) bs) (part::acc) *) *)
-      (*                end in *)
-      (*   aux (bnodes g) hm [::]. *)
-
-      (* Record partition := mkPartition { *)
-      (*                        bnodes : seq term ; *)
-      (*                        bnodes_r_bnodes : all is_bnode bnodes ; *)
-      (*                        hm : hashmap ; *)
-
-
-      (*                      }. *)
-
-      Definition is_trivial (part : part) : bool :=
-        size part == 1.
-
-      Definition is_non_trivial (part : part) : bool :=
-        ~~ is_trivial part.
-
-      Definition is_fine (p : partition) : bool :=
-        all is_trivial p.
-
-      Definition is_coarse (p : partition) : bool :=
-        size p == 1.
-
-      Definition is_intermediate (p : partition) :=
-        ~~ is_fine p && ~~ is_coarse p.
-
-
-
-      (* Definition lt_part (part1 part2 : part) : bool := *)
-      (*   if size part1 < size part2 then *)
-      (*     true *)
-      (*   else if size part1 == size part2 then *)
-
-
-      (*          Definition le_partition (p1 p2 : partition) : bool :=  *)
-      (*          fun T : Type => T -> pred T *)
-      (*                                eq_refl. *)
-      (*          . *)
-      (*          Definition partition_LePOrderMixin := LePOrderMixin partition. *)
-      (*          forall (T : eqType) (le lt : rel T), *)
-      (*   (forall x y : T, lt x y = (y != x) && le x y) -> *)
-      (*   reflexive le -> antisymmetric le -> transitive le -> lePOrderMixin T *)
-
-      
-    End Partition. *)
-
-  End IsoCanAlgorithm.
-  (* Hypothesis rdf_total_order   *)
+End IsoCanAlgorithm.
+(* Hypothesis rdf_total_order   *)
 
 End IsoCan.
 
